ulib/LowStar.Buffer.fsti
@@ -513,6 +513,19 @@ val abuffer_disjoint_intro (#t1 #t2: Type) (b1: buffer t1) (b2: buffer t2) : Lem
     abuffer_disjoint #r #a (abuffer_of_buffer b1) (abuffer_of_buffer b2)
   ))
 
+val liveness_preservation_intro
+  (#t: Type) (h h' : HS.mem) (b: buffer t)
+  (f: (
+    (t' : Type) ->
+    (pre: Preorder.preorder t') ->
+    (r: HS.mreference t' pre) ->
+    Lemma
+    (requires (HS.frameOf r == frameOf b /\ HS.as_addr r == as_addr b /\ h `HS.contains` r))
+    (ensures (h' `HS.contains` r))
+  ))
+: Lemma
+  (requires (live h b))
+  (ensures (live h' b))
 
 (* Basic, non-compositional modifies clauses, used only to implement the generic modifies clause. DO NOT USE in client code *)
 
