ulib/LowStar.Modifies.fsti
@@ -505,6 +505,48 @@ val modifies_buffer_elim
     [ SMTPat (modifies p h h'); SMTPat (B.live h' b) ]
   ] ]
 
+
+/// Some memory locations are tagged as liveness-insensitive: the
+/// liveness preservation of a memory location only depends on its
+/// disjointness from the liveness-sensitive memory locations of a
+/// modifies clause.
+
+val liveness_insensitive (l: loc) : GTot Type0
+
+val liveness_insensitive_buffer (#t: Type) (b: B.buffer t) : Lemma
+  (liveness_insensitive (loc_buffer b))
+  [SMTPat (liveness_insensitive (loc_buffer b))]
+
+val liveness_insensitive_addresses (r: HS.rid) (a: Set.set nat) : Lemma
+  (liveness_insensitive (loc_addresses true r a))
+  [SMTPat (liveness_insensitive (loc_addresses true r a))]
+
+val liveness_insensitive_union (l1 l2: loc) : Lemma
+  (liveness_insensitive (loc_union l1 l2) <==> (liveness_insensitive l1 /\ liveness_insensitive l2))
+  [SMTPat (liveness_insensitive (loc_union l1 l2))]
+
+val modifies_liveness_insensitive_mreference
+  (l1 l2 : loc)
+  (h h' : HS.mem)
+  (#t: Type)
+  (#pre: Preorder.preorder t)
+  (x: HS.mreference t pre)
+: Lemma
+  (requires (modifies (loc_union l1 l2) h h' /\ loc_disjoint l1 (loc_mreference x) /\ liveness_insensitive l2 /\ h `HS.contains` x))
+  (ensures (h' `HS.contains` x))
+  (* TODO: pattern *)
+
+val modifies_liveness_insensitive_buffer
+  (l1 l2 : loc)
+  (h h' : HS.mem)
+  (#t: Type)
+  (x: B.buffer t)
+: Lemma
+  (requires (modifies (loc_union l1 l2) h h' /\ loc_disjoint l1 (loc_buffer x) /\ liveness_insensitive l2 /\ B.live h x))
+  (ensures (B.live h' x))
+  (* TODO: pattern *)
+
+
 /// If the memory state does not change, then any memory location is
 /// modified (and, in particular, the empty set, ``loc_none``.)
 
